LeanMachinesExamples/MQueue/Bounded.lean
@@ -18,21 +18,21 @@ instance: Machine BoundedCtx (Bounded ctx) where
 
 def Init : InitEvent (Bounded ctx) Unit Unit :=
   newInitEvent'' {
-    init := { count := 0 }
+    init _ := { count := 0 }
     safety := fun _ => by simp [Machine.invariant]
   }
 
 def Incr : OrdinaryEvent (Bounded ctx) Unit Unit :=
   newEvent'' {
     guard m := m.count < ctx.maxCount
-    action m := { m with count := m.count + 1 }
+    action m _ := { m with count := m.count + 1 }
     safety := fun m => by simp [Machine.invariant] ; intro _ Hgrd ; exact Hgrd
   }
 
 def Decr : OrdinaryEvent (Bounded ctx) Unit Unit :=
   newEvent'' {
     guard m := m.count > 0
-    action m := { m with count := m.count - 1 }
+    action m _ := { m with count := m.count - 1 }
     safety := fun m => by simp [Machine.invariant] ; omega
   }
 
